DeBruijnSSA.lean
@@ -1,2 +1,3 @@
 import DeBruijnSSA.SingleApp.Syntax
 import DeBruijnSSA.SingleApp.Typing
+import DeBruijnSSA.SingleApp.Subst
