DeBruijnSSA/SingleApp/Subst.lean
@@ -1,0 +1,19 @@
+import DeBruijnSSA.SingleApp.Typing
+
+namespace SingleApp
+
+section Subst
+
+variable
+  [Φ: InstSet φ (Ty α) ε] [PartialOrder α] [PartialOrder ε] [Zero ε]
+  {Γ Δ : Ctx α ε} {σ : Subst φ}
+
+def Subst.WfD (Γ Δ : Ctx α ε) (σ : Subst φ) : Type _
+  := ∀i : Fin Δ.length, (σ i).WfD Γ (Δ.get i)
+
+def Ctx.Var.Subst (hσ : σ.WfD Γ Δ) (h : Δ.Var n V) : (σ n).WfD Γ V
+  := (hσ ⟨n, h.length⟩).wk_res h.get
+
+end Subst
+
+end SingleApp
